Use python script for withdrawal root

EvmYul/EllipticCurvesPy/rlp.py
@@ -1,0 +1,506 @@
+"""
+.. _rlp:
+
+Recursive Length Prefix (RLP) Encoding
+^^^^^^^^^^^^^^^^^^^^^^^^^^^^^^^^^^^^^^
+
+.. contents:: Table of Contents
+    :backlinks: none
+    :local:
+
+Introduction
+------------
+
+Defines the serialization and deserialization format used throughout Ethereum.
+"""
+
+# from dataclasses import astuple, fields, is_dataclass
+from typing import Any, List, Sequence, Tuple, Type, TypeVar, Union, cast
+
+from hash import Hash32, keccak256
+from exceptions import RLPDecodingError, RLPEncodingError
+
+from base_types import Bytes, Bytes0, Bytes20, FixedBytes, FixedUint, Uint
+
+RLP = Any
+
+
+#
+# RLP Encode
+#
+
+
+def encode(raw_data: RLP) -> Bytes:
+    """
+    Encodes `raw_data` into a sequence of bytes using RLP.
+
+    Parameters
+    ----------
+    raw_data :
+        A `Bytes`, `Uint`, `Uint256` or sequence of `RLP` encodable
+        objects.
+
+    Returns
+    -------
+    encoded : `ethereum.base_types.Bytes`
+        The RLP encoded bytes representing `raw_data`.
+    """
+    if isinstance(raw_data, (bytearray, bytes)):
+        return encode_bytes(raw_data)
+    elif isinstance(raw_data, (Uint, FixedUint)):
+        return encode(raw_data.to_be_bytes())
+    elif isinstance(raw_data, str):
+        return encode_bytes(raw_data.encode())
+    elif isinstance(raw_data, bool):
+        if raw_data:
+            return encode_bytes(b"\x01")
+        else:
+            return encode_bytes(b"")
+    elif isinstance(raw_data, Sequence):
+        return encode_sequence(raw_data)
+    elif is_dataclass(raw_data):
+        return encode(astuple(raw_data))
+    else:
+        raise RLPEncodingError(
+            "RLP Encoding of type {} is not supported".format(type(raw_data))
+        )
+
+
+def encode_bytes(raw_bytes: Bytes) -> Bytes:
+    """
+    Encodes `raw_bytes`, a sequence of bytes, using RLP.
+
+    Parameters
+    ----------
+    raw_bytes :
+        Bytes to encode with RLP.
+
+    Returns
+    -------
+    encoded : `ethereum.base_types.Bytes`
+        The RLP encoded bytes representing `raw_bytes`.
+    """
+    len_raw_data = Uint(len(raw_bytes))
+
+    if len_raw_data == 1 and raw_bytes[0] < 0x80:
+        return raw_bytes
+    elif len_raw_data < 0x38:
+        return bytes([0x80 + len_raw_data]) + raw_bytes
+    else:
+        # length of raw data represented as big endian bytes
+        len_raw_data_as_be = len_raw_data.to_be_bytes()
+        return (
+            bytes([0xB7 + len(len_raw_data_as_be)])
+            + len_raw_data_as_be
+            + raw_bytes
+        )
+
+
+def encode_sequence(raw_sequence: Sequence[RLP]) -> Bytes:
+    """
+    Encodes a list of RLP encodable objects (`raw_sequence`) using RLP.
+
+    Parameters
+    ----------
+    raw_sequence :
+            Sequence of RLP encodable objects.
+
+    Returns
+    -------
+    encoded : `ethereum.base_types.Bytes`
+        The RLP encoded bytes representing `raw_sequence`.
+    """
+    joined_encodings = get_joined_encodings(raw_sequence)
+    len_joined_encodings = Uint(len(joined_encodings))
+
+    if len_joined_encodings < 0x38:
+        return Bytes([0xC0 + len_joined_encodings]) + joined_encodings
+    else:
+        len_joined_encodings_as_be = len_joined_encodings.to_be_bytes()
+        return (
+            Bytes([0xF7 + len(len_joined_encodings_as_be)])
+            + len_joined_encodings_as_be
+            + joined_encodings
+        )
+
+
+def get_joined_encodings(raw_sequence: Sequence[RLP]) -> Bytes:
+    """
+    Obtain concatenation of rlp encoding for each item in the sequence
+    raw_sequence.
+
+    Parameters
+    ----------
+    raw_sequence :
+        Sequence to encode with RLP.
+
+    Returns
+    -------
+    joined_encodings : `ethereum.base_types.Bytes`
+        The concatenated RLP encoded bytes for each item in sequence
+        raw_sequence.
+    """
+    return b"".join(encode(item) for item in raw_sequence)
+
+
+#
+# RLP Decode
+#
+
+
+def decode(encoded_data: Bytes) -> RLP:
+    """
+    Decodes an integer, byte sequence, or list of RLP encodable objects
+    from the byte sequence `encoded_data`, using RLP.
+
+    Parameters
+    ----------
+    encoded_data :
+        A sequence of bytes, in RLP form.
+
+    Returns
+    -------
+    decoded_data : `RLP`
+        Object decoded from `encoded_data`.
+    """
+    if len(encoded_data) <= 0:
+        raise RLPDecodingError("Cannot decode empty bytestring")
+
+    if encoded_data[0] <= 0xBF:
+        # This means that the raw data is of type bytes
+        return decode_to_bytes(encoded_data)
+    else:
+        # This means that the raw data is of type sequence
+        return decode_to_sequence(encoded_data)
+
+
+T = TypeVar("T")
+
+
+def decode_to(cls: Type[T], encoded_data: Bytes) -> T:
+    """
+    Decode the bytes in `encoded_data` to an object of type `cls`. `cls` can be
+    a `Bytes` subclass, a dataclass, `Uint`, `U256` or `Tuple[cls]`.
+
+    Parameters
+    ----------
+    cls: `Type[T]`
+        The type to decode to.
+    encoded_data :
+        A sequence of bytes, in RLP form.
+
+    Returns
+    -------
+    decoded_data : `T`
+        Object decoded from `encoded_data`.
+    """
+    return _decode_to(cls, decode(encoded_data))
+
+
+def _decode_to(cls: Type[T], raw_rlp: RLP) -> T:
+    """
+    Decode the rlp structure in `encoded_data` to an object of type `cls`.
+    `cls` can be a `Bytes` subclass, a dataclass, `Uint`, `U256`,
+    `Tuple[cls, ...]`, `Tuple[cls1, cls2]` or `Union[Bytes, cls]`.
+
+    Parameters
+    ----------
+    cls: `Type[T]`
+        The type to decode to.
+    raw_rlp :
+        A decoded rlp structure.
+
+    Returns
+    -------
+    decoded_data : `T`
+        Object decoded from `encoded_data`.
+    """
+    if isinstance(cls, type(Tuple[Uint, ...])) and cls._name == "Tuple":  # type: ignore # noqa: E501
+        if not isinstance(raw_rlp, list):
+            raise RLPDecodingError
+        if cls.__args__[1] == ...:  # type: ignore
+            args = []
+            for raw_item in raw_rlp:
+                args.append(_decode_to(cls.__args__[0], raw_item))  # type: ignore # noqa: E501
+            return tuple(args)  # type: ignore
+        else:
+            args = []
+            if len(raw_rlp) != len(cls.__args__):  # type: ignore
+                raise RLPDecodingError
+            for t, raw_item in zip(cls.__args__, raw_rlp):  # type: ignore
+                args.append(_decode_to(t, raw_item))
+            return tuple(args)  # type: ignore
+    elif cls == Union[Bytes0, Bytes20]:
+        if not isinstance(raw_rlp, Bytes):
+            raise RLPDecodingError
+        if len(raw_rlp) == 0:
+            return Bytes0()  # type: ignore
+        elif len(raw_rlp) == 20:
+            return Bytes20(raw_rlp)  # type: ignore
+        else:
+            raise RLPDecodingError(
+                "Bytes has length {}, expected 0 or 20".format(len(raw_rlp))
+            )
+    elif isinstance(cls, type(List[Bytes])) and cls._name == "List":  # type: ignore # noqa: E501
+        if not isinstance(raw_rlp, list):
+            raise RLPDecodingError
+        items = []
+        for raw_item in raw_rlp:
+            items.append(_decode_to(cls.__args__[0], raw_item))  # type: ignore
+        return items  # type: ignore
+    elif isinstance(cls, type(Union[Bytes, List[Bytes]])) and cls.__origin__ == Union:  # type: ignore # noqa: E501
+        if len(cls.__args__) != 2 or Bytes not in cls.__args__:  # type: ignore
+            raise RLPDecodingError(
+                "RLP Decoding to type {} is not supported".format(cls)
+            )
+        if isinstance(raw_rlp, Bytes):
+            return raw_rlp  # type: ignore
+        elif cls.__args__[0] == Bytes:  # type: ignore
+            return _decode_to(cls.__args__[1], raw_rlp)  # type: ignore
+        else:
+            return _decode_to(cls.__args__[0], raw_rlp)  # type: ignore
+    elif issubclass(cls, bool):
+        if raw_rlp == b"\x01":
+            return cls(True)  # type: ignore
+        elif raw_rlp == b"":
+            return cls(False)  # type: ignore
+        else:
+            raise TypeError("Cannot decode {} as {}".format(raw_rlp, cls))
+    elif issubclass(cls, FixedBytes):
+        if not isinstance(raw_rlp, Bytes):
+            raise RLPDecodingError
+        if len(raw_rlp) != cls.LENGTH:
+            raise RLPDecodingError
+        return cls(raw_rlp)  # type: ignore
+    elif issubclass(cls, Bytes):
+        if not isinstance(raw_rlp, Bytes):
+            raise RLPDecodingError
+        return raw_rlp  # type: ignore
+    elif issubclass(cls, (Uint, FixedUint)):
+        if not isinstance(raw_rlp, Bytes):
+            raise RLPDecodingError
+        try:
+            return cls.from_be_bytes(raw_rlp)  # type: ignore
+        except ValueError:
+            raise RLPDecodingError
+    elif is_dataclass(cls):
+        if not isinstance(raw_rlp, list):
+            raise RLPDecodingError
+        assert isinstance(raw_rlp, list)
+        args = []
+        if len(fields(cls)) != len(raw_rlp):
+            raise RLPDecodingError
+        for field, rlp_item in zip(fields(cls), raw_rlp):
+            args.append(_decode_to(field.type, rlp_item))
+        return cast(T, cls(*args))
+    else:
+        raise RLPDecodingError(
+            "RLP Decoding to type {} is not supported".format(cls)
+        )
+
+
+def decode_to_bytes(encoded_bytes: Bytes) -> Bytes:
+    """
+    Decodes a rlp encoded byte stream assuming that the decoded data
+    should be of type `bytes`.
+
+    Parameters
+    ----------
+    encoded_bytes :
+        RLP encoded byte stream.
+
+    Returns
+    -------
+    decoded : `ethereum.base_types.Bytes`
+        RLP decoded Bytes data
+    """
+    if len(encoded_bytes) == 1 and encoded_bytes[0] < 0x80:
+        return encoded_bytes
+    elif encoded_bytes[0] <= 0xB7:
+        len_raw_data = encoded_bytes[0] - 0x80
+        if len_raw_data >= len(encoded_bytes):
+            raise RLPDecodingError
+        raw_data = encoded_bytes[1 : 1 + len_raw_data]
+        if len_raw_data == 1 and raw_data[0] < 0x80:
+            raise RLPDecodingError
+        return raw_data
+    else:
+        # This is the index in the encoded data at which decoded data
+        # starts from.
+        decoded_data_start_idx = 1 + encoded_bytes[0] - 0xB7
+        if decoded_data_start_idx - 1 >= len(encoded_bytes):
+            raise RLPDecodingError
+        if encoded_bytes[1] == 0:
+            raise RLPDecodingError
+        len_decoded_data = Uint.from_be_bytes(
+            encoded_bytes[1:decoded_data_start_idx]
+        )
+        if len_decoded_data < 0x38:
+            raise RLPDecodingError
+        decoded_data_end_idx = decoded_data_start_idx + len_decoded_data
+        if decoded_data_end_idx - 1 >= len(encoded_bytes):
+            raise RLPDecodingError
+        return encoded_bytes[decoded_data_start_idx:decoded_data_end_idx]
+
+
+def decode_to_sequence(encoded_sequence: Bytes) -> List[RLP]:
+    """
+    Decodes a rlp encoded byte stream assuming that the decoded data
+    should be of type `Sequence` of objects.
+
+    Parameters
+    ----------
+    encoded_sequence :
+        An RLP encoded Sequence.
+
+    Returns
+    -------
+    decoded : `Sequence[RLP]`
+        Sequence of objects decoded from `encoded_sequence`.
+    """
+    if encoded_sequence[0] <= 0xF7:
+        len_joined_encodings = encoded_sequence[0] - 0xC0
+        if len_joined_encodings >= len(encoded_sequence):
+            raise RLPDecodingError
+        joined_encodings = encoded_sequence[1 : 1 + len_joined_encodings]
+    else:
+        joined_encodings_start_idx = 1 + encoded_sequence[0] - 0xF7
+        if joined_encodings_start_idx - 1 >= len(encoded_sequence):
+            raise RLPDecodingError
+        if encoded_sequence[1] == 0:
+            raise RLPDecodingError
+        len_joined_encodings = Uint.from_be_bytes(
+            encoded_sequence[1:joined_encodings_start_idx]
+        )
+        if len_joined_encodings < 0x38:
+            raise RLPDecodingError
+        joined_encodings_end_idx = (
+            joined_encodings_start_idx + len_joined_encodings
+        )
+        if joined_encodings_end_idx - 1 >= len(encoded_sequence):
+            raise RLPDecodingError
+        joined_encodings = encoded_sequence[
+            joined_encodings_start_idx:joined_encodings_end_idx
+        ]
+
+    return decode_joined_encodings(joined_encodings)
+
+
+def decode_joined_encodings(joined_encodings: Bytes) -> List[RLP]:
+    """
+    Decodes `joined_encodings`, which is a concatenation of RLP encoded
+    objects.
+
+    Parameters
+    ----------
+    joined_encodings :
+        concatenation of RLP encoded objects
+
+    Returns
+    -------
+    decoded : `List[RLP]`
+        A list of objects decoded from `joined_encodings`.
+    """
+    decoded_sequence = []
+
+    item_start_idx = 0
+    while item_start_idx < len(joined_encodings):
+        encoded_item_length = decode_item_length(
+            joined_encodings[item_start_idx:]
+        )
+        if item_start_idx + encoded_item_length - 1 >= len(joined_encodings):
+            raise RLPDecodingError
+        encoded_item = joined_encodings[
+            item_start_idx : item_start_idx + encoded_item_length
+        ]
+        decoded_sequence.append(decode(encoded_item))
+        item_start_idx += encoded_item_length
+
+    return decoded_sequence
+
+
+def decode_item_length(encoded_data: Bytes) -> int:
+    """
+    Find the length of the rlp encoding for the first object in the
+    encoded sequence.
+    Here `encoded_data` refers to concatenation of rlp encoding for each
+    item in a sequence.
+
+    NOTE - This is a helper function not described in the spec. It was
+    introduced as the spec doesn't discuss about decoding the RLP encoded
+    data.
+
+    Parameters
+    ----------
+    encoded_data :
+        RLP encoded data for a sequence of objects.
+
+    Returns
+    -------
+    rlp_length : `int`
+    """
+    if len(encoded_data) <= 0:
+        raise RLPDecodingError
+
+    first_rlp_byte = Uint(encoded_data[0])
+
+    # This is the length of the big endian representation of the length of
+    # rlp encoded object byte stream.
+    length_length = Uint(0)
+    decoded_data_length = 0
+
+    # This occurs only when the raw_data is a single byte whose value < 128
+    if first_rlp_byte < 0x80:
+        # We return 1 here, as the end formula
+        # 1 + length_length + decoded_data_length would be invalid for
+        # this case.
+        return 1
+    # This occurs only when the raw_data is a byte stream with length < 56
+    # and doesn't fall into the above cases
+    elif first_rlp_byte <= 0xB7:
+        decoded_data_length = first_rlp_byte - 0x80
+    # This occurs only when the raw_data is a byte stream and doesn't fall
+    # into the above cases
+    elif first_rlp_byte <= 0xBF:
+        length_length = first_rlp_byte - 0xB7
+        if length_length >= len(encoded_data):
+            raise RLPDecodingError
+        if encoded_data[1] == 0:
+            raise RLPDecodingError
+        decoded_data_length = Uint.from_be_bytes(
+            encoded_data[1 : 1 + length_length]
+        )
+    # This occurs only when the raw_data is a sequence of objects with
+    # length(concatenation of encoding of each object) < 56
+    elif first_rlp_byte <= 0xF7:
+        decoded_data_length = first_rlp_byte - 0xC0
+    # This occurs only when the raw_data is a sequence of objects and
+    # doesn't fall into the above cases.
+    elif first_rlp_byte <= 0xFF:
+        length_length = first_rlp_byte - 0xF7
+        if length_length >= len(encoded_data):
+            raise RLPDecodingError
+        if encoded_data[1] == 0:
+            raise RLPDecodingError
+        decoded_data_length = Uint.from_be_bytes(
+            encoded_data[1 : 1 + length_length]
+        )
+
+    return 1 + length_length + decoded_data_length
+
+
+def rlp_hash(data: RLP) -> Hash32:
+    """
+    Obtain the keccak-256 hash of the rlp encoding of the passed in data.
+
+    Parameters
+    ----------
+    data :
+        The data for which we need the rlp hash.
+
+    Returns
+    -------
+    hash : `Hash32`
+        The rlp hash of the passed in data.
+    """
+    return keccak256(encode(data))
