EvmYul/State/Withdrawal.lean
@@ -1,4 +1,7 @@
+-- Requires the following python packages: pycryptodome
+
 import EvmYul.Wheels
+import EvmYul.PerformIO
 import Conform.Wheels
 
 open EvmYul ByteArray
@@ -22,17 +25,89 @@ def to𝕋 : Withdrawal → 𝕋
 
 end Withdrawal
 
-private def someWithdrawal : Withdrawal :=
-  { index := 0
-  , validatorIndex := 1
-  , recipient := 0x00000000219ab540356cbb839cbe05303d7705fa
-  , amount := 2
+def blobComputeTrieRoot (ws : List (String × String)) : String :=
+  totallySafePerformIO ∘ IO.Process.run <|
+    pythonCommandOfInput ws
+  where pythonCommandOfInput (ws : List (String × String)) : IO.Process.SpawnArgs := {
+    cmd := "python3",
+    args :=
+      #["EvmYul/EllipticCurvesPy/withdrawal.py"]
+        ++ #[ws.length.repr]
+        ++ .mk (List.join ∘ List.map (λ (i, w) ↦ [i, w]) <| ws)
   }
 
-#eval RLP someWithdrawal.to𝕋 |>.map ByteArray.data
+def toBlobs (w : Withdrawal) : Option (String × String) := do
+  let rlpᵢ ← RLP (.𝔹 (BE w.index.val))
+  let rlp ← RLP w.to𝕋
+  pure (EvmYul.toHex rlpᵢ, EvmYul.toHex rlp)
 
-example :
-  (RLP someWithdrawal.to𝕋).map ByteArray.data
+-- EIP-4895
+def computeTrieRoot (ws : List Withdrawal) : Except String ByteArray := do
+  match List.traverse toBlobs ws with
+    | none => .error "Could not encode withdrawal."
+    | some ws => ByteArray.ofBlob (blobComputeTrieRoot ws)
+
+-- Tests
+
+private def withdrawal₁ : Withdrawal :=
+  { index := 0x00
+  , validatorIndex := 0x00
+  , recipient := 0x6295ee1b4f6dd65047762f924ecd367c17eabf8f
+  , amount := 0x01
+  }
+
+private def withdrawal₂ : Withdrawal :=
+  { index := 0x00
+  , validatorIndex := 0x00
+  , recipient := 0x000f3df6d732807ef1319fb7b8bb8522d0beac02
+  , amount := 0x01
+  }
+
+private def withdrawal₃ : Withdrawal :=
+  { index := 0x01
+  , validatorIndex := 0x01
+  , recipient := 0xfffffffffffffffffffffffffffffffffffffffe
+  , amount := 0x01
+  }
+
+private def withdrawalZeroTrailingRoot : Withdrawal :=
+  { index := 0x00
+  , validatorIndex := 0x00
+  , recipient := 0x0000000000000000000000000000000000000001
+  , amount := 0x00
+  }
+
+private example :
+  (computeTrieRoot []).toOption
+    ==
+  (ByteArray.ofBlob
+    "56e81f171bcc55a6ff8345e692c0f86e5b48e01b996cadc001622fb5e363b421"
+  ).toOption
+:= by native_decide
+
+/- From newly_created_contract.json -/
+private example :
+  (computeTrieRoot [withdrawal₁]).toOption
     =
-  some #[216, 128, 1, 148, 0, 0, 0, 0, 33, 154, 181, 64, 53, 108, 187, 131, 156, 190, 5, 48, 61, 119, 5, 250, 2]
+  (ByteArray.ofBlob
+    "82cc6fbe74c41496b382fcdf25216c5af7bdbb5a3929e8f2e61bd6445ab66436"
+  ).toOption
+:= by native_decide
+
+/- From beacon_root_contract_deploy.json -/
+private example :
+  (computeTrieRoot [withdrawal₂, withdrawal₃]).toOption
+    =
+  (ByteArray.ofBlob
+    "2aef4d3e6939af0b4bf4c0e7572a214eb7db9ba52937e1e82ad6c64b52d2e8bb"
+  ).toOption
+:= by native_decide
+
+/- From withdrawing_to_precompiles.json -/
+private example :
+  (computeTrieRoot [withdrawalZeroTrailingRoot]).toOption
+    =
+  (ByteArray.ofBlob
+    "04cc2e3f94b587ff46b5f4c0787c589db306b7209f7f212f47022a12bc3e6e16"
+  ).toOption
 := by native_decide
